Starting cleanup and movement of core libs.
This commit includes changes to Logic.ec (with their consequences),
and changes to FMap (with their consequences). FMap still needs
extended.

Changes made here do not appear in the update script.

tests/prhl/success/0015-upto-2.ec
@@ -1,6 +1,6 @@
 require import Distr.
 require import FSet.
-require import Map. 
+require import FMap.
 require import Int.
 
 module type O = { 
@@ -17,7 +17,7 @@ module RO = {
   proc hash (x:int) : int = { 
     var r : int;
     r = $[0..10];
-    if (!in_dom x mH) mH.[x] = r;
+    if (!mem x (dom mH)) mH.[x] = r;
     return (proj mH.[x]);
   }
 
@@ -40,7 +40,7 @@ module F1(A:Adv) = {
   proc main() : int = { 
     var h: int;
     var r : int;
-    RO.mH    = Map.empty;
+    RO.mH    = FMap.empty;
     RO.logA  = FSet.empty;
     h        = RO.hash(xs);
     r        = A1.a(h);
@@ -56,7 +56,7 @@ module F2(A:Adv) = {
   proc main() : int = { 
     var h: int;
     var r : int;
-    RO.mH    = Map.empty;
+    RO.mH    = FMap.empty;
     RO.logA  = FSet.empty;
     h        = $[0..10];
     r        = A1.a(h);
@@ -77,7 +77,9 @@ proof -strict.
             (RO.logA{1} = RO.logA{2} /\ F1.xs{1} = F2.xs{2} /\
             eq_except RO.mH{1} RO.mH{2} F2.xs{2}),  
             (F1.xs{1} = F2.xs{2})).
-    proc; inline RO.hash;wp;rnd;wp;skip;simplify;smt.
+timeout 10.
+    proc; inline RO.hash;wp;rnd;wp;skip;simplify; progress=> //; smt.
+timeout 3.
 
     (* Hoare goal *)
     intros &2 h.
